Write case proved

txn-data-consistency/Prot_2PC_2PL.thy
@@ -670,6 +670,132 @@ next
   qed simp
 qed
 
+text\<open>Invariants about status of TM\<close>
+definition InitInv where
+  "InitInv s k \<longleftrightarrow> (\<forall>t. km_status (kms s k) t = working \<longrightarrow> tm_status (tm s (get_cl_txn t)) \<in> {tm_init, tm_prepared})"
+
+lemmas InitInvI = InitInv_def[THEN iffD2, rule_format]
+lemmas InitInvE[elim] = InitInv_def[THEN iffD1, elim_format, rule_format]
+
+lemma reach_initinv [simp, intro]: "reach tps s \<Longrightarrow> InitInv s k"
+proof(induction s arbitrary: k rule: reach.induct)
+  case (reach_init s)
+  then show ?case
+  by (auto simp add: InitInv_def tps_defs)
+next
+  case (reach_trans s e s')
+  then show ?case 
+  proof (cases e)
+    case (Write2 x11 x12 x13)
+    then show ?thesis sorry
+  next
+    case (Read2 x21 x22 x23)
+    then show ?thesis sorry
+  next
+    case (Prepare x31 x32)
+    then show ?thesis sorry
+  next
+    case (RLock x41 x42)
+    then show ?thesis sorry
+  next
+    case (WLock x51 x52)
+    then show ?thesis sorry
+  next
+    case (NoLock x61 x62)
+    then show ?thesis sorry
+  next
+    case (NOK x71 x72)
+    then show ?thesis sorry
+  next
+    case (Commit x81 x82)
+    then show ?thesis sorry
+  next
+    case (Abort x91 x92)
+    then show ?thesis sorry
+  next
+    case (User_Commit x10)
+    then show ?thesis sorry
+  next
+    case (TM_Commit x111 x112 x113 x114)
+    then show ?thesis sorry
+  next
+    case (TM_Abort x12a)
+    then show ?thesis sorry
+  next
+    case (TM_ReadyC x13a)
+    then show ?thesis sorry
+  next
+    case (TM_ReadyA x14)
+    then show ?thesis sorry
+  next
+    case Skip2
+    then show ?thesis sorry
+  qed
+qed
+
+definition PreparedInv where
+  "PreparedInv s k \<longleftrightarrow> (\<forall>t. km_status (kms s k) t = prepared \<longrightarrow> tm_status (tm s (get_cl_txn t)) = tm_prepared)"
+
+lemmas PreparedInvI = PreparedInv_def[THEN iffD2, rule_format]
+lemmas PreparedInvE[elim] = PreparedInv_def[THEN iffD1, elim_format, rule_format]
+
+lemma reach_preparedinv [simp, intro]: "reach tps s \<Longrightarrow> PreparedInv s k"
+proof(induction s arbitrary: k rule: reach.induct)
+  case (reach_init s)
+  then show ?case
+  by (auto simp add: PreparedInv_def tps_defs)
+next
+  case (reach_trans s e s')
+  then show ?case 
+  proof (cases e)
+    case (Write2 x11 x12 x13)
+    then show ?thesis sorry
+  next
+    case (Read2 x21 x22 x23)
+    then show ?thesis sorry
+  next
+    case (Prepare x31 x32)
+    then show ?thesis sorry
+  next
+    case (RLock x41 x42)
+    then show ?thesis sorry
+  next
+    case (WLock x51 x52)
+    then show ?thesis sorry
+  next
+    case (NoLock x61 x62)
+    then show ?thesis sorry
+  next
+    case (NOK x71 x72)
+    then show ?thesis sorry
+  next
+    case (Commit x81 x82)
+    then show ?thesis sorry
+  next
+    case (Abort x91 x92)
+    then show ?thesis sorry
+  next
+    case (User_Commit x10)
+    then show ?thesis sorry
+  next
+    case (TM_Commit x111 x112 x113 x114)
+    then show ?thesis sorry
+  next
+    case (TM_Abort x12a)
+    then show ?thesis sorry
+  next
+    case (TM_ReadyC x13a)
+    then show ?thesis sorry
+  next
+    case (TM_ReadyA x14)
+    then show ?thesis sorry
+  next
+    case Skip2
+    then show ?thesis sorry
+  qed
+qed
+
+
 text\<open>Invariants about Fingerprint being empty after a commit/abort\<close>
 definition TCCommitEmpF where
   "TCCommitEmpF s cl k \<longleftrightarrow> (tm_status (tm s cl) = tm_committed
@@ -939,16 +1065,22 @@ definition update_kv_reads_all_txn :: "(txid0 \<Rightarrow> status_tm) \<Rightar
     (let lv = last_version vl uk in
      vl [Max uk :=
        lv \<lparr>v_readerset := (v_readerset lv)
-          \<union> {t.\<exists>v. tFk t R = Some v \<and> tStm t = tm_committed \<and> tSkm t \<in> {read_lock, write_lock}}\<rparr>])"
+          \<union> {t. tStm t = tm_committed \<and> tSkm t \<in> {read_lock, write_lock} \<and> tFk t R \<noteq> None}\<rparr>])"
 
 abbreviation the_wr_t :: "(txid0 \<Rightarrow> status_km) \<Rightarrow> txid0" where
   "the_wr_t tSkm \<equiv> (THE t. tSkm t = write_lock)"
+
+lemma the_wr_tI:
+  assumes "km_status (kms s k) t = write_lock"
+      and "WLockInv s k"
+  shows "the_wr_t (km_status (kms s k)) = t"
+  using assms
+  by blast
 
 definition update_kv_writes_all_txn :: "(txid0 \<Rightarrow> status_tm) \<Rightarrow> (txid0 \<Rightarrow> status_km) \<Rightarrow>
   (txid0 \<Rightarrow> 'v key_fp) \<Rightarrow> 'v v_list \<Rightarrow> 'v v_list" where
   "update_kv_writes_all_txn tStm tSkm tFk vl =
     (if (\<exists>t. tStm t = tm_committed \<and> tSkm t = write_lock) then
-    \<comment> \<open>(\<forall>t. tSkm t \<noteq> write_lock) then vl else (if tStm (the_wr_t tSkm) = tm_committed then\<close>
         update_kv_writes (the_wr_t tSkm) (tFk (the_wr_t tSkm)) vl
      else vl)"
 
@@ -994,8 +1126,8 @@ lemma [simp]: "Max {..<Suc 0} = 0" by (auto simp add: lessThan_def)
 
 lemma tps_refines_et_es: "tps \<sqsubseteq>\<^sub>med ET_SER.ET_ES"
 proof (intro simulate_ES_fun_with_invariant[where I="\<lambda>s. \<forall>cl k. TIDFutureKm s cl \<and> TCInit s cl \<and>
-  TCPrepared s cl \<and> TCCommitted s cl \<and> TCAborted s cl \<and> TCCommitEmpF s cl k \<and> TCAbortEmpF s cl k \<and>
-  RLockInv s k \<and> WLockInv s k"])
+  TCPrepared s cl \<and> TCCommitted s cl \<and> TCAborted s cl \<and> InitInv s k \<and> PreparedInv s k \<and>
+  TCCommitEmpF s cl k \<and> TCAbortEmpF s cl k \<and> RLockInv s k \<and> WLockInv s k"])
   fix gs0
   assume p: "init tps gs0"
   then show "init ET_SER.ET_ES (sim gs0)" using p
@@ -1005,19 +1137,38 @@ next
   fix gs a gs'
   assume p: "tps: gs\<midarrow>a\<rightarrow> gs'"
      and inv: "\<forall>cl k. TIDFutureKm gs cl \<and> TCInit gs cl \<and> TCPrepared gs cl \<and> TCCommitted gs cl \<and>
-                      TCAborted gs cl \<and> TCCommitEmpF gs cl k \<and> TCAbortEmpF gs cl k \<and>
-                      RLockInv gs k \<and> WLockInv gs k"
+                      TCAborted gs cl \<and> InitInv gs k \<and>  PreparedInv gs k \<and> TCCommitEmpF gs cl k \<and>
+                      TCAbortEmpF gs cl k \<and> RLockInv gs k \<and> WLockInv gs k"
   then show "ET_SER.ET_ES: sim gs\<midarrow>med a\<rightarrow> sim gs'"
   proof (cases a)
     case (Write2 x11 x12 x13)
     hence "\<forall>x t. a \<noteq> Commit x t" by auto
-    hence "\<forall>k. km_vl (kms gs' k) = km_vl (kms gs k)" using km_vl_inv p by blast
-    hence "kvs_of_gs gs' = kvs_of_gs gs" using Write2 p inv
-      apply (auto simp add: tps_trans_defs unchanged_defs sim_def kvs_of_gs_def update_kv_all_defs)
-      apply (rule ext) subgoal for k
-      apply (cases "\<exists>t. tm_status (tm gs (get_cl_txn t)) = tm_committed \<and> km_status (kms gs k) t = write_lock"; simp) sorry done
-    then show ?thesis using Write2 p
-      by (auto simp add: tps_trans_defs unchanged_defs sim_def views_of_gs_def)
+    hence v: "\<forall>k. km_vl (kms gs' k) = km_vl (kms gs k)" using km_vl_inv p by blast
+    hence "\<forall>k t. km_status (kms gs' k) t = km_status (kms gs k) t" using p Write2
+      apply (auto simp add: write2_def unchanged_defs)
+      subgoal for k t by(cases "k = x11"; cases "t = x12"; simp).
+    hence s: "\<forall>k. km_status (kms gs' k) = km_status (kms gs k)" by (auto simp add: fun_eq_iff)
+    hence c: "tm_status (tm gs (get_cl_txn x12)) \<noteq> tm_committed" using inv p Write2
+      apply (auto simp add: tps_trans_defs)
+      by (metis InitInv_def insertE singleton_iff status_tm.distinct(3) status_tm.distinct(7))
+    hence r: "\<And>k t. (tm_status (tm gs (get_cl_txn t)) = tm_committed \<and>
+                   (km_status (kms gs k) t = read_lock \<or> km_status (kms gs k) t = write_lock) \<and>
+                    km_key_fp (kms gs' k) t R \<noteq> None) =
+                   (tm_status (tm gs (get_cl_txn t)) = tm_committed \<and>
+                   (km_status (kms gs k) t = read_lock \<or> km_status (kms gs k) t = write_lock) \<and>
+                    km_key_fp (kms gs k) t R \<noteq> None)"
+      using Write2 p subgoal for k t
+        apply (cases "t = x12"; simp add: tps_trans_defs unchanged_defs) by metis.
+    have w:"\<forall>k vl. update_kv_writes_all_txn (\<lambda>t. tm_status (tm gs (get_cl_txn t)))
+                (km_status (kms gs k)) (km_key_fp (kms gs' k)) vl =
+               update_kv_writes_all_txn (\<lambda>t. tm_status (tm gs (get_cl_txn t)))
+                (km_status (kms gs k)) (km_key_fp (kms gs k)) vl"
+      using Write2 p c v s inv
+      apply (auto simp add: update_kv_writes_all_txn_def update_kv_writes_def)
+      subgoal for k vl t
+        by (cases "k = x11"; cases "t = x12"; simp add: tps_trans_defs unchanged_defs the_wr_tI).
+    then show ?thesis using Write2 p v s r w
+      by (auto simp add: tps_trans_defs unchanged_defs sim_defs)
   next
     case (Read2 x21 x22 x23)
     then show ?thesis using p inv
